Phi_Semantics/PhiSem_Aggregate_Tuple.thy
@@ -16,7 +16,7 @@ debt_axiomatization T_tup :: \<open>TY list type_entry\<close>
 
 interpretation tuple_ty TY_CONS_OF \<open>TYPE(TY_N)\<close> \<open>TYPE(TY)\<close> T_tup using tuple_ty_ax .
 
-(*TODO: intergrate the hidding into the automation command*)
+(*TODO: intergrate automatic hidding into the automation command*)
 hide_fact tuple_ty_ax
 
 subsubsection \<open>Value\<close>
@@ -34,6 +34,8 @@ hide_fact tuple_val_ax
 
 abbreviation \<open>tup \<equiv> tup.mk\<close>
 
+term \<open>tuple(a, b, c, d)\<close>
+
 subsection \<open>Semantics\<close>
 
 debt_axiomatization
@@ -42,10 +44,10 @@ debt_axiomatization
   and   V_tup_sep_disj_R[simp]: \<open>V_tup.mk l1 ## vl2 \<longleftrightarrow> (\<exists>l2. vl2 = V_tup.mk l2)\<close>
   and   V_tup_sep_disj_L[simp]: \<open>vl1 ## V_tup.mk l2 \<longleftrightarrow> (\<exists>l1. vl1 = V_tup.mk l1)\<close>
   and   V_tup_mult    : \<open>V_tup.mk l1 * V_tup.mk l2 = V_tup.mk (l2 @ l1)\<close>
-  and   idx_step_type_tup [eval_semantic_index] : \<open>i < length tys \<Longrightarrow> idx_step_type i (tup tys) = tys!i \<close>
-  and   valid_idx_step_tup[eval_semantic_index] : \<open>valid_idx_step (tup tys) i \<longleftrightarrow> i < length tys\<close>
-  and   idx_step_value_tup[eval_semantic_index] : \<open>idx_step_value i (V_tup.mk vs) = vs!i\<close>
-  and   idx_step_mod_value_tup : \<open>idx_step_mod_value i f (V_tup.mk vs) = V_tup.mk (vs[i := f (vs!i)])\<close>
+  and   idx_step_type_tup [eval_semantic_index] : \<open>i < length tys \<Longrightarrow> idx_step_type (AgIdx_N i) (tup tys) = tys!i \<close>
+  and   valid_idx_step_tup[eval_semantic_index] : \<open>valid_idx_step (tup tys) j \<longleftrightarrow> j \<in> {AgIdx_N i | i. i < length tys}\<close>
+  and   idx_step_value_tup[eval_semantic_index] : \<open>idx_step_value (AgIdx_N i) (V_tup.mk vs) = vs!i\<close>
+  and   idx_step_mod_value_tup : \<open>idx_step_mod_value (AgIdx_N i) f (V_tup.mk vs) = V_tup.mk (vs[i := f (vs!i)])\<close>
 
 lemma V_tup_mult_cons:
   \<open>NO_MATCH vs ([]::VAL list) \<Longrightarrow> V_tup.mk (v#vs) = V_tup.mk vs * V_tup.mk [v]\<close>
@@ -64,23 +66,24 @@ section \<open>\<phi>Type\<close>
 
 subsection \<open>Empty Tuple\<close>
 
-definition EmptyTuple :: \<open>(VAL, unit) \<phi>\<close>
-  where \<open>EmptyTuple x = { V_tup.mk [] }\<close>
+definition Empty_Tuple :: \<open>(VAL, unit) \<phi>\<close>
+  where \<open>Empty_Tuple x = { V_tup.mk [] }\<close>
+
+\<phi>adhoc_overloading \<phi>_Empty_Tuple_sugar Empty_Tuple
 
 lemma EmptyTuple_expn[\<phi>expns]:
-  \<open>p \<in> (x \<Ztypecolon> EmptyTuple) \<longleftrightarrow> p = V_tup.mk []\<close>
-  unfolding EmptyTuple_def \<phi>Type_def by simp
+  \<open>p \<in> (x \<Ztypecolon> Empty_Tuple) \<longleftrightarrow> p = V_tup.mk []\<close>
+  unfolding Empty_Tuple_def \<phi>Type_def by simp
 
 subsection \<open>Field\<close>
 
 definition Tuple_Field :: "(VAL, 'a) \<phi> \<Rightarrow> (VAL, 'a) \<phi>"
   where "Tuple_Field T x = { V_tup.mk [v] |v. v \<in> T x }"
 
-syntax "_\<phi>Tuple" :: \<open>tuple_args \<Rightarrow> logic\<close> ("\<lbrace> _ \<rbrace>")
+syntax "\<phi>_tuple_" :: \<open>logic \<Rightarrow> \<phi>_tuple_arg_\<close> ("_")
 
 translations
-  "_\<phi>Tuple (_tuple_arg X)" \<rightleftharpoons> "CONST Tuple_Field X"
-  "_\<phi>Tuple (_tuple_args y z)" \<rightleftharpoons> "CONST \<phi>Prod (_\<phi>Tuple (_tuple_arg y)) (_\<phi>Tuple z)"
+  "_\<phi>Tuple (_\<phi>tuple_arg (\<phi>_tuple_ X))" \<rightleftharpoons> "CONST Tuple_Field X"
 
 lemma Tuple_Field_expn[\<phi>expns]:
   \<open>p \<in> (x \<Ztypecolon> \<lbrace> T \<rbrace>) \<longleftrightarrow> (\<exists>v. p = V_tup.mk [v] \<and> v \<in> (x \<Ztypecolon> T))\<close>
@@ -90,9 +93,9 @@ lemma Tuple_Field_inhabited[elim!,\<phi>inhabitance_rule]:
   \<open>Inhabited (x \<Ztypecolon> \<lbrace> T \<rbrace>) \<Longrightarrow> (Inhabited (x \<Ztypecolon> T) \<Longrightarrow> C) \<Longrightarrow> C\<close>
   unfolding Inhabited_def by (simp add: \<phi>expns)
 
-lemma EmptyTuple_reduce[simp]:
-  \<open>(((),a) \<Ztypecolon> EmptyTuple \<^emph> \<lbrace> T \<rbrace>) = (a \<Ztypecolon> \<lbrace> T \<rbrace>)\<close>
-  \<open>((a,()) \<Ztypecolon> \<lbrace> T \<rbrace> \<^emph> EmptyTuple) = (a \<Ztypecolon> \<lbrace> T \<rbrace>)\<close>
+lemma Empty_Tuple_reduce[simp]:
+  \<open>(((),a) \<Ztypecolon> Empty_Tuple \<^emph> \<lbrace> T \<rbrace>) = (a \<Ztypecolon> \<lbrace> T \<rbrace>)\<close>
+  \<open>((a,()) \<Ztypecolon> \<lbrace> T \<rbrace> \<^emph> Empty_Tuple) = (a \<Ztypecolon> \<lbrace> T \<rbrace>)\<close>
   unfolding set_eq_iff
   apply (clarsimp; rule; clarsimp simp add: \<phi>expns V_tup_mult)
   apply (metis V_tup_mult append_Nil)
@@ -137,61 +140,56 @@ lemma [\<phi>reason 1200]:
   \<open> \<c>\<o>\<n>\<d>\<i>\<t>\<i>\<o>\<n> i < length Tys
 \<Longrightarrow> Simplify eval_semantic_index Ty (Tys!i) 
 \<Longrightarrow> valid_index Ty L
-\<Longrightarrow> valid_index (tup Tys) (i#L)\<close>
+\<Longrightarrow> valid_index (tup Tys) (AgIdx_N i # L)\<close>
   unfolding Premise_def Simplify_def
   by (simp add: valid_idx_step_tup idx_step_type_tup)
 
 subsection \<open>Index\<close>
 
 lemma idx_step_value_V_tup_suc:
-  \<open>idx_step_value (Suc i) (V_tup.mk (va # vs)) = idx_step_value i (V_tup.mk vs)\<close>
+  \<open>idx_step_value (AgIdx_N (Suc i)) (V_tup.mk (va # vs)) = idx_step_value (AgIdx_N i) (V_tup.mk vs)\<close>
   by (simp add: idx_step_value_tup)
 
 lemma idx_step_mod_value_V_tup_suc:
-  \<open>idx_step_mod_value (Suc i) g (V_tup.mk (va # vs)) = idx_step_mod_value i g (V_tup.mk vs) * V_tup.mk [va]\<close>
+  \<open>idx_step_mod_value (AgIdx_N (Suc i)) g (V_tup.mk (va # vs)) = idx_step_mod_value (AgIdx_N i) g (V_tup.mk vs) * V_tup.mk [va]\<close>
   by (metis NO_MATCH_I V_tup_mult_cons idx_step_mod_value_tup list_update_code(3) nth_Cons_Suc)
 
-declare [[\<phi>trace_reasoning = 1]]
-
 lemma [\<phi>reason 1200]:
-  \<open> \<phi>Index_getter (i # idx) X Y f
-\<Longrightarrow> \<phi>Index_getter (Suc i # idx) (\<lbrace> T \<rbrace> \<^emph> X) Y (f o snd)\<close>
+  \<open> \<phi>Index_getter (AgIdx_N i # idx) X Y f
+\<Longrightarrow> \<phi>Index_getter (AgIdx_N (Suc i) # idx) (\<lbrace> T \<rbrace> \<^emph> X) Y (f o snd)\<close>
   unfolding \<phi>Index_getter_def
   by (clarsimp simp add: \<phi>expns V_tup_mult idx_step_value_V_tup_suc)
 
 lemma [\<phi>reason 1200]:
   \<open> \<phi>Index_getter idx X Y f
-\<Longrightarrow> \<phi>Index_getter (0 # idx) \<lbrace> X \<rbrace> Y f\<close>
+\<Longrightarrow> \<phi>Index_getter (AgIdx_N 0 # idx) \<lbrace> X \<rbrace> Y f\<close>
   unfolding \<phi>Index_getter_def
   by (clarsimp simp add: \<phi>expns V_tup_mult idx_step_value_tup)
 
 lemma [\<phi>reason 1200]:
   \<open> \<phi>Index_getter idx X Y f
-\<Longrightarrow> \<phi>Index_getter (0 # idx) (\<lbrace> X \<rbrace> \<^emph> R) Y (f o fst)\<close>
+\<Longrightarrow> \<phi>Index_getter (AgIdx_N 0 # idx) (\<lbrace> X \<rbrace> \<^emph> R) Y (f o fst)\<close>
   unfolding \<phi>Index_getter_def
   by (clarsimp simp add: \<phi>expns V_tup_mult idx_step_value_tup)
 
 lemma [\<phi>reason 1200]:
-  \<open> \<phi>Index_mapper (i # idx) X X' Y Y' f
-\<Longrightarrow> \<phi>Index_mapper (Suc i # idx) (\<lbrace> T \<rbrace> \<^emph> X) (\<lbrace> T \<rbrace> \<^emph> X') Y Y' (apsnd o f)\<close>
+  \<open> \<phi>Index_mapper (AgIdx_N i # idx) X X' Y Y' f
+\<Longrightarrow> \<phi>Index_mapper (AgIdx_N (Suc i) # idx) (\<lbrace> T \<rbrace> \<^emph> X) (\<lbrace> T \<rbrace> \<^emph> X') Y Y' (apsnd o f)\<close>
   unfolding \<phi>Index_mapper_def
   apply (clarsimp simp add: \<phi>expns V_tup_mult idx_step_mod_value_V_tup_suc)
   by (metis V_tup_sep_disj_R idx_step_mod_value_tup)
 
 lemma [\<phi>reason 1200]:
   \<open> \<phi>Index_mapper idx X X' Y Y' f
-\<Longrightarrow> \<phi>Index_mapper (0 # idx) \<lbrace> X \<rbrace> \<lbrace> X' \<rbrace> Y Y' f\<close>
+\<Longrightarrow> \<phi>Index_mapper (AgIdx_N 0 # idx) \<lbrace> X \<rbrace> \<lbrace> X' \<rbrace> Y Y' f\<close>
   unfolding \<phi>Index_mapper_def
   by (clarsimp simp add: \<phi>expns V_tup_mult idx_step_mod_value_tup)
 
 lemma [\<phi>reason 1200]:
   \<open> \<phi>Index_mapper idx X X' Y Y' f
-\<Longrightarrow> \<phi>Index_mapper (0 # idx) (\<lbrace> X \<rbrace> \<^emph> R) (\<lbrace> X' \<rbrace> \<^emph> R) Y Y' (apfst o f)\<close>
+\<Longrightarrow> \<phi>Index_mapper (AgIdx_N 0 # idx) (\<lbrace> X \<rbrace> \<^emph> R) (\<lbrace> X' \<rbrace> \<^emph> R) Y Y' (apfst o f)\<close>
   unfolding \<phi>Index_mapper_def
   apply (clarsimp simp add: \<phi>expns V_tup_mult idx_step_mod_value_tup)
   by (metis NO_MATCH_def V_tup_mult_cons V_tup_sep_disj_L)
-
-
-
 
 end
