Phi_Semantics/PhiSem_Aggregate_Path.thy
@@ -1,0 +1,63 @@
+theory PhiSem_Aggregate_Path
+  imports PhiSem_Base PhiTool_Symbol
+begin
+
+section \<open>Path of Elements in an Aggregate Structure\<close>
+
+datatype 'val aggregate_index' = AgIdx_N nat | AgIdx_S symbol | AgIdx_V 'val
+
+type_synonym aggregate_index = \<open>VAL aggregate_index'\<close>
+type_synonym aggregate_path = \<open>aggregate_index list\<close>
+
+nonterminal "\<phi>_ag_idx_"
+
+syntax "_ID_ag_idx_"  :: \<open>\<phi>_symbol_ \<Rightarrow> \<phi>_ag_idx_\<close> ("_")
+       "_0_ag_idx_"   :: \<open>\<phi>_ag_idx_\<close> ("0")
+       "_1_ag_idx_"   :: \<open>\<phi>_ag_idx_\<close> ("1")
+       "_num_ag_idx_" :: \<open>num_token \<Rightarrow> \<phi>_ag_idx_\<close> ("_")
+       "_log_ag_idx_" :: \<open>logic \<Rightarrow> \<phi>_ag_idx_\<close> ("LOGIC'(_')")
+       "_MK_ag_idx_"  :: \<open>\<phi>_ag_idx_ \<Rightarrow> aggregate_index\<close> ("\<phi>AG'_IDX'(_')")
+
+ML \<open>
+structure Phi_Aggregate_Syntax = struct
+
+fun parse_index (Const(\<^syntax_const>\<open>_ID_ag_idx_\<close> , _) $ id) =
+        Const(\<^const_name>\<open>AgIdx_S\<close>, dummyT) $ (Const(\<^const_name>\<open>mk_symbol\<close>, dummyT) $ id)
+  | parse_index (Const(\<^syntax_const>\<open>_num_ag_idx_\<close>, _) $ Free (n, _)) =
+        Const(\<^const_name>\<open>AgIdx_N\<close>, dummyT) $ mk_numeral_nat (Value.parse_nat n)
+  | parse_index (Const(\<^syntax_const>\<open>_log_ag_idx_\<close>, _) $ tm) = tm
+  | parse_index (Const(\<^syntax_const>\<open>_0_ag_idx_\<close>, _)) =
+        Const(\<^const_name>\<open>AgIdx_N\<close>, dummyT) $ mk_numeral_nat 0
+  | parse_index (Const(\<^syntax_const>\<open>_1_ag_idx_\<close>, _)) =
+        Const(\<^const_name>\<open>AgIdx_N\<close>, dummyT) $ mk_numeral_nat 1
+  | parse_index x = (@{print} x; error "SYNTAX ERROR #ee2e77a2-b6d7-4acf-ae18-5d266dc2f06e")
+
+fun print_index (Const(\<^const_syntax>\<open>AgIdx_S\<close>, _) $ (Const(\<^const_syntax>\<open>mk_symbol\<close>, _) $ tm)) =
+     (case Phi_Tool_Symbol.revert_symbol (dest_synt_numeral tm)
+        of SOME id => Free(id, dummyT)
+         | NONE => tm)
+  | print_index (Const (\<^const_syntax>\<open>AgIdx_N\<close>, _) $ tm) =
+      Free(string_of_int (dest_synt_numeral tm), dummyT)
+  | print_index tm = Const(\<^syntax_const>\<open>_log_ag_idx_\<close>, dummyT) $ tm
+
+end
+\<close>
+
+parse_translation \<open>[
+  (\<^syntax_const>\<open>_MK_ag_idx_\<close>, fn ctxt => fn [x] => Phi_Aggregate_Syntax.parse_index x)
+]\<close>
+
+print_translation \<open>[
+  (\<^const_syntax>\<open>AgIdx_S\<close>, (fn ctxt => fn [Const(\<^const_syntax>\<open>mk_symbol\<close>, _) $ tm] =>
+      case Phi_Tool_Symbol.revert_symbol (dest_synt_numeral tm)
+        of SOME id => Const (\<^syntax_const>\<open>_MK_ag_idx_\<close>, dummyT) $ Free(id, dummyT)
+         | NONE => tm)),
+  (\<^const_syntax>\<open>AgIdx_N\<close>, (fn ctxt => fn [tm] =>
+      case try dest_synt_numeral tm
+        of SOME N => Const (\<^syntax_const>\<open>_MK_ag_idx_\<close>, dummyT) $ Free(string_of_int N, dummyT)))
+]\<close>
+
+
+
+
+end
