Phi_Semantics/PhiTool_Symbol.thy
@@ -1,0 +1,58 @@
+theory PhiTool_Symbol
+  imports Main
+begin
+
+section \<open>Symbol Identifier unique in Isabelle Runtime and Its Persistent Image\<close>
+
+text \<open>When the runtime system has N symbols in total, the length of the representation
+  is at most 2 + log2(N).
+TODO: don't use nat but make a numeral so we don't need the mk_symbol wrapper\<close>
+
+typedef symbol = \<open>UNIV::nat set\<close>
+  morphisms Abs_symbol mk_symbol
+  by auto
+
+hide_const Abs_symbol
+
+declare mk_symbol_inject[simplified, iff]
+
+ML_file \<open>PhiTool_Symbol_syntax.ML\<close>
+ML_file \<open>PhiTool_Symbol.ML\<close>
+
+nonterminal "\<phi>_symbol_"
+
+syntax "_ID_SYMBOL_" :: \<open>id \<Rightarrow> \<phi>_symbol_\<close> ("_")
+       "_LOG_EXPR_SYMBOL_" :: \<open>logic \<Rightarrow> \<phi>_symbol_\<close> ("LOGIC'(_')")
+       "_MK_SYMBOL_" :: \<open>\<phi>_symbol_ \<Rightarrow> symbol\<close> ("SYMBOL'(_')")
+
+declare [[ML_debugger]]
+
+ML \<open>
+structure Phi_Tool_Symbol = struct
+open Phi_Tool_Symbol
+
+fun parse (Free (id, _)) = Phi_Tool_Symbol.mk_symbol id
+  | parse tm = (@{print} tm; error "Expect an identifier.")
+
+fun print tm =
+  case Option.map Phi_Tool_Symbol.revert_symbol (try dest_synt_numeral tm)
+    of SOME (SOME id) => Free(id, dummyT)
+     | SOME NONE => error ("Phi_Tool_Symbol: " ^ string_of_int (dest_synt_numeral tm) ^ " is not a known symbol!")
+     | NONE => tm
+
+end
+\<close>
+
+parse_translation \<open>[
+  (\<^syntax_const>\<open>_ID_SYMBOL_\<close>, (fn ctxt => fn [x] => Phi_Tool_Symbol.parse x)),
+  (\<^syntax_const>\<open>_MK_SYMBOL_\<close>, (fn ctxt =>
+    (fn [Const(\<^syntax_const>\<open>_LOG_EXPR_SYMBOL_\<close>, _) $ x] => x
+      | [x] => Const(\<^const_name>\<open>mk_symbol\<close>, dummyT) $ x)))
+]\<close>
+
+print_translation \<open>[
+  (\<^const_syntax>\<open>mk_symbol\<close>, (fn ctxt => fn [tm] => Const (\<^syntax_const>\<open>_MK_SYMBOL_\<close>, dummyT) $ Phi_Tool_Symbol.print tm))
+]\<close>
+
+
+end
