Phi_Test/PhiTest_All_Sem.thy
@@ -6,6 +6,10 @@ theory PhiTest_All_Sem
           Phi_Semantics.PhiSem_Variable
           Phi_Semantics.PhiSem_Int_ArbiPrec
           Phi_Semantics.PhiSem_Machine_Integer
+          Phi_Semantics.PhiSem_Mem_Pointer
+          Phi_Semantics.PhiSem_Aggregate_Array
+          Phi_Semantics.PhiSem_Aggregate_Tuple
+          Phi_Semantics.PhiSem_Aggregate_Named_Tuple
           (*Phi_Semantics.PhiSem_Mem_OO TO BE FIXED*)
 begin
 
